[WIP] check

theories/check1.v
@@ -6,7 +6,7 @@ From HB Require Import structures.
 
 Set Implicit Arguments.
 
-Lemma TODO: False. Admitted.
+Axiom TODO: False.
 Ltac TODO := exfalso; apply TODO.
 
 Notation typecheck := option.
@@ -202,6 +202,9 @@ End has_cut.
 
 Definition full_sP {K:eqType} {V:Type} (s: list (K*V)) := forall k, lookup k s <> None.
 Notation sigV := (list (V * S)).
+
+Axiom valid_sigA: forall (A:sigV), valid_sig A.
+Ltac vst:= apply: valid_sigA.
 
 Section min_max.
     Definition maxD (d1 d2 : D) :=
@@ -680,6 +683,31 @@ Section min_max.
         rewrite (not_incl_strong _ _ _ M2) (not_incl_strong _ _ _ M1)//.
   Qed.
 
+  Lemma incl_arrP {m A B C D}:
+    incl (arr m A B) (arr m C D) =
+      map_ty_bool (if m == o then incl A C else incl C A)
+      (incl B D).
+  Proof.
+    rewrite/incl/=.
+    case: m => //=.
+    rewrite -/not_incl not_incl_incl//.
+  Qed.
+
+  Lemma incl_weak1 {A}: incl A (weak A) = ty_ok true
+  with not_incl_strong1 {A}: not_incl A (strong A) = ty_ok true.
+  Proof.
+    - case: A.
+        clear; move=> []//[]//.
+      move=> []s1 s2; rewrite /=incl_arrP/=.
+        rewrite incl_weak1 incl_not_incl not_incl_strong1//.
+      rewrite !incl_weak1//.
+    case: A.
+      clear; move=> []//[]//.
+    move=> []s1 s2; rewrite not_incl_incl /=incl_arrP/=.
+      rewrite incl_weak1 incl_not_incl not_incl_strong1//.
+    rewrite !incl_not_incl !not_incl_strong1//.
+  Qed.
+
   Lemma weak_strong {A B}: weak A = weak B -> strong A = strong B
   with strong_weak {A B}: strong A = strong B -> weak A = weak B.
   Proof.
@@ -853,84 +881,76 @@ Section checker.
     end.
 
   Definition any:= (b (d Pred), false).
+  Definition anyT:= (b (d Pred), true).
+
+  Definition checkr s2 b2 tl tr :=
+    match incl s2 tl with
+    | ty_ok true => if b2 then (tr, true) else (weak tr, false)
+    | ty_ok false | ty_err => (weak tr, false)
+    end.
 
   (* takes a tm and returns its signature + if it is well-called
      the tm has no signature if its head is a variable with no assignment in sV *)
   Fixpoint check_tm (sP:sigT) (sV:sigV) (tm : Tm) : S * bool :=
     match tm with
     | Tm_Kd k => ((b Exp, true))
-    | Tm_Kp k => odflt any (omap (fun x => (x, true)) (lookup k sP))
-    | Tm_V v => odflt any (omap (fun x => (x, true)) (lookup v sV))
+    | Tm_Kp k => odflt anyT (omap (fun x => (x, true)) (lookup k sP))
+    | Tm_V v => odflt anyT (omap (fun x => (x, true)) (lookup v sV))
     | Tm_Comb l r => 
         let checkl := check_tm sP sV l in
         match checkl with
         | (arr i tl tr, b1) => 
-          let checkr := check_tm sP sV r in
-          match checkr with
-          | (s2, b2) =>
-            match incl s2 tl with
-            | ty_ok true => if b1 && b2 then (tr, true) else (weak tr, false)
-            | ty_ok false | ty_err => (weak tr, false)
-            end
-          end
+          if tl == weak tl then (tr, true)
+          else if b1 == false then (weak tr, false)
+          else
+            let (cr, br) := check_tm sP sV r in
+            checkr cr br tl tr
         | (arr o tl tr, b1) => (tr, b1)
-        | _ => any
+        | _ => anyT
         end
-    end.
-
-  Definition squash_to_D S :=
-    match S with
-    | (b _, _) as X => X
-    | (_, gc) => any
     end.
 
   (* takes a tm and a signature and updates variable signatures
      updates are performed only on toplevel variables or variables in input positions *)
-  Fixpoint assume_tm (sP:sigT) (sV:sigV) (tm : Tm) (s : S): typecheck sigV :=
+  Fixpoint assume_tm (sP:sigT) (sV:sigV) (tm : Tm) (s : S): sigV :=
     match tm with
-    | Tm_Kd _ | Tm_Kp _ => ty_ok sV (*TODO: should I raise ty_err if mismatch between s and type(tm)? *)
+    | Tm_Kd _ | Tm_Kp _ => sV (*TODO: should I raise ty_err if mismatch between s and type(tm)? *)
     | Tm_V v =>
-      if lookup v sV is Some s' then map_ty (fun s'' => ty_ok (add v s'' sV)) (min s s')
-      else ty_ok (add v s sV)
+      if lookup v sV is Some s' then
+        match min s s' with
+        | None => add v s sV
+        | Some s'' => (add v s'' sV)
+        end
+      else (add v s sV)
     | Tm_Comb l r =>
       match s with
       | arr i tl tr =>
-        map_ty (fun sP' => assume_tm sP sP' r tr) (assume_tm sP sV l tl)
+        (fun sP' => assume_tm sP sP' r tr) (assume_tm sP sV l tl)
       | arr o tl tr => assume_tm sP sV l tl
-      | _ => ty_err
+      | _ => sV
       end
     end.
 
   (* assumes the output tm and then it goes on inputs *)
-  Fixpoint assume_call (sP:sigT) (sV:sigV) (c : Callable) (s : S): typecheck sigV :=
-    match c with
-    | Callable_Kp _ => ty_ok sV (*TODO: should I raise ty_err if mismatch between s and type(c)? *)
-    | Callable_V v => ty_ok sV
-    | Callable_Comb l r =>
-      match s with
-      | arr i tl tr => assume_call sP sV l tl
-      | arr o tl tr => 
-        map_ty (fun sV' => assume_tm sP sV' r tr) (assume_call sP sV l tl)
-      | _ => ty_err
-      end
-    end.
+  Definition assume_call (sP:sigT) (sV:sigV) (c : Callable) (s : S): sigV :=
+    assume_tm sP sV (Callable2Tm c) s.
 
   (* assumes variables in input positions *)
-  Fixpoint assume_hd (sP:sigT) (sV:sigV) (s : S) (tm:Tm) : typecheck sigV :=
+  Fixpoint assume_hd (sP:sigT) (sV:sigV) (s : S) (tm:Tm) : sigV :=
     match tm with
-    | Tm_Kd _ => ty_ok sV
-    | Tm_Kp _ => ty_ok sV
+    | Tm_Kd _ => sV
+    | Tm_Kp _ => sV
     | Tm_V v =>
       if lookup v sV is Some s' then
-        map_ty (fun s'' => ty_ok (add v s'' sV)) (min s s')
+        odflt sV (omap (fun s'' => (add v s'' sV)) (min s s'))
       else 
-        ty_ok (add v s sV)
+        (add v s sV)
     | Tm_Comb l r => 
       match s with
       | arr i tl tr => 
-        map_ty (fun sV' => assume_hd sP sV' tr r) (assume_hd sP sV tl l)
+        (fun sV' => assume_hd sP sV' tr r) (assume_hd sP sV tl l)
       | arr o tl _ => (assume_hd sP sV tl l)
-      | _ => ty_err
+      | _ => sV
       end
     end.
 
@@ -960,12 +980,11 @@ Section checker.
   (* checks inputs and assumes outputs of a callable *)
   Definition check_callable sP sV (c: Callable) d : (D * sigV)%type :=
     match check_tm sP sV (Callable2Tm c)  with
-    (* | ty_err => (Pred, sV) *)
     | (((b Exp | arr _ _ _), _)) => (Pred, sV) (*NOTE: callable have type prop!*)
     | (b(d x), b1) =>
       if b1 then 
         if get_callable_hd_sig sP sV c is Some s then
-          odflt ((Pred, sV)) (omap (fun sV' => (maxD x d, sV')) (assume_call sP sV c s))
+          (maxD x d, (assume_call sP sV c s))
         else (Pred, sV)
       else (Pred, sV)
     end.
@@ -989,7 +1008,6 @@ Section checker.
   (* The rules passes the check if:
      - it is implementing a function or a relation, the body is function, the outputs are ok
   *)
-  (* Set Printing All. *)
   Definition check_rule sP sV head prems : bool :=
     let hd_sig := RCallable_sig sP head in
     match hd_sig with
@@ -998,13 +1016,9 @@ Section checker.
         let is_det_head := is_det_sig hd_sig in
         let tm_head := (Callable2Tm (RCallable2Callable head)) in
         let ass_hd := assume_hd sP sV hd_sig tm_head in
-        match ass_hd with
-        | None => false
-        | Some sV' =>
-          let: (b1, sV'') := check_atoms sP sV' prems Func in
-            if is_det_head && (b1 == Pred) then false
-            else odflt false (check_hd sP sV'' hd_sig tm_head)
-          end
+        let: (b1, sV'') := check_atoms sP ass_hd prems Func in
+          if is_det_head && (b1 == Pred) then false
+          else odflt false (check_hd sP sV'' hd_sig tm_head)
     end.
 
   Definition check_rules sP sV rules : bool :=
@@ -1013,6 +1027,14 @@ Section checker.
   Definition check_program sP := 
     forall pr, check_rules sP empty_ctx (rules pr).
 End checker.
+
+Lemma checkr_weak_tr s2 b2 tl tr x b: 
+  checkr s2 b2 tl (weak tr) = (x, b) -> weak tr = x.
+Proof.
+  rewrite /checkr.
+  case I: incl => [[] |]; [|move=> [<-]; rewrite weak2//..].
+  destruct b2; move=> [<-]; rewrite ?weak2//.
+Qed.
 
 Lemma check_callable_pred {sP sV c d1 d2 s}:
   check_callable sP sV c d1 = (d2, s) ->
@@ -1023,8 +1045,8 @@ Proof.
   have ?: (Pred, sV) = (d2, s) -> maxD d2 d1 = d2 by move=> [<-].
   case C: check_tm => /=[[[|x []]|]]//.
   case gc: get_callable_hd_sig => [S|]; [|move=>[<-//]].
-  case ac: assume_call => //=[sV'].
-  move=> [<-]; rewrite -maxD_assoc maxD_refl//.
+  move=> [??]; subst.
+  rewrite -maxD_assoc maxD_refl//.
 Qed.
 
 Definition full_ko A:= (next_alt false A == None).
@@ -1043,10 +1065,11 @@ Section merge.
         map_ty' (fun m => add k m s) (max v e)
     end.
 
-  Fixpoint merge_sig1 (s1 s2: sigV) : typecheck (sigV) :=
+  Fixpoint merge_sig1 (s1 s2: sigV) : (sigV) :=
     match s2 with
-    | [::] => ty_ok s1
-    | x::xs => map_ty (fun (s1':sigV) => merge_sig1 s1' xs) (update s1 x)
+    | [::] => s1
+    | x::xs => 
+      merge_sig1 (odflt s1 (update s1 x)) xs
     end.
 
   Definition weak_bf_merge (s1 s2: sigV) : sigV :=  
@@ -1125,11 +1148,11 @@ Section merge.
   Qed.
 
   Lemma merge_refl {A}: 
-    valid_sig A -> merge_sig A A = ty_ok A.
+    valid_sig A -> merge_sig A A = A.
   Proof. TODO. Qed.
 
   Lemma valid_sig_merge {A B C}:
-    valid_sig A -> valid_sig B -> merge_sig A B = ty_ok C -> valid_sig C.
+    valid_sig A -> valid_sig B -> merge_sig A B = C -> valid_sig C.
   Proof. TODO. Qed.
 
   Lemma weak_all_add {k v C}:
@@ -1140,8 +1163,8 @@ Section merge.
     rewrite IH//.
   Qed.
 
-  Lemma merge_add {xs k v C D}:
-    merge_sig (add k v C) xs = ty_ok D ->
+  (* Lemma merge_add {xs k v C D}:
+    merge_sig (add k v C) xs = D ->
       exists x, lookup k D = Some x /\ incl v x = ty_ok true.
   Proof.
     rewrite/merge_sig.
@@ -1152,7 +1175,7 @@ Section merge.
       apply: weak_incl.
     - move=> [k v] xs IH C D k1 v1/=.
       TODO.
-  Qed.
+  Qed. *)
 
   Lemma merge_comm {A B}: merge_sig A B = merge_sig B A.
   Proof.
@@ -1165,8 +1188,11 @@ Section merge.
     valid_sig B -> valid_sig C ->
     lookup k B = Some kB ->
     lookup k C = Some kC ->
-    merge_sig B C = ty_ok D ->
-    exists kD, max kB kC = ty_ok kD /\ lookup k D = Some kD.
+    merge_sig B C = D ->
+    match max kB kC with
+    | ty_ok kD => max kB kC = ty_ok kD /\ lookup k D = Some kD
+    | ty_err => lookup k D = None
+    end.
   Proof.
     elim: C B D k kB kC => //=[[k v] xs IH] B D k' kB kC H1/= /andP[].
     rewrite/key_absent.
@@ -1184,54 +1210,11 @@ Section merge.
     TODO.
   Qed.
 
-  Lemma compat_type_merge_lookup {A B C} k:
-    valid_sig A ->
-    merge_sig A B = ty_ok C ->
-      match lookup k C with
-      | None => lookup k A = None /\ lookup k B = None
-      | Some vC => 
-        match lookup k A with
-        | None => omap weak (lookup k B) = Some vC
-        | Some vA => 
-          match lookup k B with
-          | None => weak vA = vC
-          | Some vB => max vA vB = ty_ok vC
-          end
-        end
-      end.
-  Proof.
-    rewrite merge_comm/=.
-    rewrite/merge_sig.
-    elim: A B C k => //=[|[k v] A IH] B C k1/=.
-      rewrite weak_bf_merge_0s => _ [<-] {C}.
-      rewrite lookup_weak_all.
-      case L: lookup => /=[vB|]//.
-    move=> /andP[+ VA].
-    rewrite/key_absent; case LA: lookup => //= _.
-    rewrite weak_bf_mergeP/=eqxx.
-    case: eqP => H; subst.
-      case L: lookup => [vB|]//=.
-        case M: max => //=[m].
-  Admitted.
-
-  Lemma merge_sig_add_compat {k vB' v A B B'}:
-    valid_sig A -> valid_sig B ->
-    merge_sig A B = ty_ok B' ->
-      lookup k B' = Some vB' -> compat_type v vB' ->
-        exists C vC, merge_sig (add k v A) B = ty_ok C /\ 
-          lookup k C = Some vC /\ 
-          match lookup k B with
-          | None => vC = weak v
-          | Some v' => max v' v = ty_ok vC
-          end .
-  Proof.  
-  Abort.
-
   Lemma merge_sig_valid_sig {A B C}:
-    valid_sig A -> valid_sig B -> merge_sig A B = ty_ok C ->
+    valid_sig A -> valid_sig B -> merge_sig A B = C ->
       valid_sig C.
   Proof.
-    rewrite/merge_sig.
+    (* rewrite/merge_sig.
     elim: B A C => //=[|[k v] A IH] B C VB/=.
       rewrite weak_bf_merge_0s => _ [<-].
       rewrite valid_sig_weal_all//.
@@ -1241,6 +1224,7 @@ Section merge.
       case M: max => //=[m].
       rewrite (@add_weak_bf_merge _ _ _ _ v)//=?eqxx//.
       TODO.
+    TODO. *)
     TODO.
   Qed.
 
@@ -1269,7 +1253,7 @@ Fixpoint tc_tree_aux (sP:sigT) (sV : sigV) A (dd:D) : (D * sigV)%type :=
       (fun '(ddB0, sB0) =>
           (fun '(ddB, sB) =>
             (fun x => 
-            (maxD ddB0 ddB, x)) (odflt sV (merge_sig sB sB0))) tcB) tcB0
+            (maxD ddB0 ddB, x)) ((merge_sig sB sB0))) tcB) tcB0
     end
   | Or A _ B =>
       if is_ko A then tc_tree_aux sP sV B dd
@@ -1280,7 +1264,7 @@ Fixpoint tc_tree_aux (sP:sigT) (sV : sigV) A (dd:D) : (D * sigV)%type :=
        (fun '(dA, sA) =>
          (fun '(dB, sB) =>
           (fun x => 
-          (if has_cut A then maxD dA dB else Pred, x)) (odflt sV (merge_sig sA sB))) tcB) tA
+          (if has_cut A then maxD dA dB else Pred, x)) ((merge_sig sA sB))) tcB) tA
   end.
 
 Section func2.
@@ -1292,8 +1276,7 @@ Section func2.
       by move=> [<-<-]; exists Pred.
     rewrite/check_callable.
     case: check_tm => //=[[[//|] d|//]][]//.
-    case: get_callable_hd_sig => // S.
-    case: assume_call => //= C [<-<-].
+    case: get_callable_hd_sig => // S [??]; subst.
     repeat eexists.
     by destruct d.
   Qed.
@@ -1356,34 +1339,31 @@ Section func2.
 End func2.
 
 Section valid_sig_preservation.
+  Axiom OK : False.
+  Ltac OK := exfalso; apply: OK.
   Lemma assume_tm_valid_sig {sP sv1 svA c S}:
     valid_sig sv1 ->
-    assume_tm sP sv1 c S = ty_ok (svA) -> valid_sig svA.
-  Proof.
-  Admitted.
+    assume_tm sP sv1 c S = (svA) -> valid_sig svA.
+  Proof. OK. Qed.
 
   Lemma assume_call_valid_sig {sP sv1 svA c S}:
     valid_sig sv1 ->
-    assume_call sP sv1 c S = ty_ok (svA) -> 
+    assume_call sP sv1 c S = (svA) -> 
       valid_sig svA.
-  Proof.
-  Admitted.
+  Proof. OK. Qed.
 
   Lemma check_callable_valid_sig {sP sv1 svA c d ign}:
     valid_sig sv1 ->
     check_callable sP sv1 c ign = (d, svA) ->
     (maxD d ign = d /\ valid_sig svA)%type2.
-  Proof.
-    Admitted.
+  Proof. OK. Qed.
 
 
   Lemma tc_tree_aux_valid_sig {sP sv1 svA A d ign}:
     valid_sig sv1 ->
     tc_tree_aux sP sv1 A ign = (d, svA) ->
     valid_sig svA.
-  Proof.
-    Admitted.
-
+  Proof. OK. Qed.
 
 End valid_sig_preservation.
 
@@ -1692,19 +1672,23 @@ Section more_precise.
     | [::] => all (fun x => x.2 == weak x.2) big
     | (k,v_small)::xs => 
       match lookup k big with
-      | None => false
-      | Some v_big => 
-        ((incl v_small v_big) == ty_ok true) && 
+      | None => more_precise xs (remove k big)
+      | Some v_big =>
+        (((incl v_small v_big) == ty_ok true) || (v_big == weak v_big)) &&
         more_precise xs (remove k big)
       end
     end.
 
-  Lemma more_precise_key_absent {k s l}:
+
+  (* Lemma more_precise_key_absent {k s l}:
     more_precise l (remove k s) -> key_absent k l.
   Proof.
     rewrite/key_absent.
     elim: l k s => //= -[k v] xs IH k' ys.
-    case x: lookup => //=[S] /andP[/eqP H1 +].
+    case x: lookup => //=[S|]; last first.
+      case:eqP => H; subst => /=.
+      rew 
+    move=> /andP[/eqP H1 +].
     case:eqP => //= H3; subst.
       by rewrite lookup_remove_None in x.
     (* move=> /IH. *)
@@ -1712,9 +1696,9 @@ Section more_precise.
     rewrite remove_comm//.
     move=> /IH.
     case L: lookup => //=.
-  Qed.
+  Qed. *)
 
-  Lemma more_precise_valid_sig {A B}:
+  (* Lemma more_precise_valid_sig {A B}:
     valid_sig B -> more_precise A B -> valid_sig A.
   Proof.
     elim: A B => /=[|[k v] A IH] B VB//.
@@ -1722,6 +1706,51 @@ Section more_precise.
     move=> /andP[/eqP I M].
     rewrite (IH _ (valid_sig_remove VB) M) andbT.
     apply: more_precise_key_absent M.
+  Qed. *)
+
+  Lemma more_precise_removel {k A B}:
+    valid_sig B ->
+    key_absent k A ->
+    more_precise A B -> more_precise A (remove k B).
+  Proof.
+    rewrite/key_absent; case L: lookup => // + _.
+    elim: A k B L => //=[|[k v] A IH] k1 B/= + VB.
+      move=> _.
+      elim: B k1 VB => //=[[k v] B IH] k1/= /andP[A1 VB] /andP[/eqP kB WB].
+      case: eqP => H; subst => /=.
+        apply: IH VB WB.
+      rewrite -kB eqxx/=.
+      by apply: IH; eauto.
+    case: eqP => //= H1 H2.
+    rewrite lookup_remove_diff; [|congruence].
+    case LB: lookup => //=[vB|]; f_equal.
+      move=> /andP[->]/=.
+      rewrite remove_comm.
+      apply: IH; auto.
+      apply: valid_sig_remove VB.
+    rewrite remove_comm key_absent_remove//.
+      apply: IH; auto.
+    by rewrite/key_absent LB.
+  Qed.
+
+  Lemma more_precise_remover {k A B}:
+    valid_sig B ->
+    key_absent k B ->
+    more_precise A B -> more_precise (remove k A) B.
+  Proof.
+    rewrite/key_absent; case L: lookup => // + _.
+    elim: A k B L => //=[[k v] A IH] k1 B/= LB VB.
+    case H: (k1 == k); move: H => /eqP H/=; subst.
+      rewrite LB/=.
+      rewrite key_absent_remove.
+        apply: IH; auto.
+      rewrite/key_absent LB//.
+    case LB1: lookup => [vB|]; last first.
+      apply: IH (valid_sig_remove VB).
+      rewrite lookup_remove_diff//; congruence.
+    move=> /andP[->]/=.
+    apply: IH (valid_sig_remove VB).
+    rewrite lookup_remove_diff//; congruence.
   Qed.
 
   Lemma more_precise_remove2 {A B} k:
@@ -1734,40 +1763,62 @@ Section more_precise.
         by apply: IH.
       rewrite -H1 eqxx/=.
       apply: IH H2.
-    case LB: lookup => //=[vB] /andP[/eqP H1 H2].
-    case: eqP => //= H; subst.
-      rewrite -(@remove2 _ _ _ B).
-      apply: IH (valid_sig_remove VB) H2.
-    rewrite lookup_remove_diff// LB H1/=.
-    rewrite remove_comm.
-    apply: IH (valid_sig_remove VB) H2.
+    case LB: lookup => //=[vB|]; last first.
+      have HH : key_absent k B by rewrite /key_absent LB.
+      case:eqP => H/=; subst.
+        rewrite key_absent_remove//=.
+        by apply: more_precise_remover.
+      rewrite lookup_remove_diff// LB.
+      rewrite remove_comm.
+      apply: IH (valid_sig_remove VB).
+    move=> /andP[].
+    case H: (k1 == k); move/eqP: H => H/=; subst.
+      move=> H H1.
+      apply: more_precise_remover; auto.
+      rewrite (valid_sig_remove)//.
+      by rewrite/key_absent lookup_remove_None.
+    move=> H1 H2.
+    rewrite lookup_remove_diff//LB H1/=.
+    by rewrite remove_comm; apply: IH (valid_sig_remove _) _.
   Qed.
 
-  Lemma more_precise_removel {k A B v}:
-    valid_sig B ->
-    key_absent k A -> lookup k B = Some (weak v) ->
-    more_precise A (remove k B) = more_precise A B.
+  Lemma more_precise_remove3 {A B k vB}:
+    valid_sig B -> lookup k B = Some (weak vB) ->
+    more_precise A (remove k B) ->
+    more_precise A B.
   Proof.
-    rewrite/key_absent; case L: lookup => // + _.
-    elim: A k B v L => //=[|[k v] A IH] k1 B/= v1 + VB.
-      move=> _ KB.
-      elim: B v1 k1 VB KB => //=[[k v] B IH] v1 k1 /= /andP[kB VB].
-      case: eqP => H; subst => /=.
-        move=> []?; subst => /=.
-        rewrite eqxx/= weak2 eqxx//=.
-        rewrite key_absent_remove//.
-      case: eqP; [congruence|] => //= _.
-      move=> H1; f_equal.
-      by apply: IH; eauto.
-    case: eqP => //= H1 H2 H3.
-    rewrite lookup_remove_diff; [|congruence].
-    case LB: lookup => //=[vB]; f_equal.
-    rewrite remove_comm//.
-    apply: IH H2 (valid_sig_remove VB) _.
-    rewrite lookup_remove_diff// H3//.
+    elim: A B k => //=[|[k v] A IH] B k1 VB.
+      elim: B k1 VB => /=[|[k v] A IH]//= k1 /andP[+VA].
+      rewrite/key_absent; case LA: lookup => // _.
+      case: eqP => //=H; subst.
+        move=> [?]; subst.
+        rewrite weak2 !eqxx/=.
+        rewrite key_absent_remove///key_absent LA//.
+      move=> H1.
+      case: eqP; [congruence|].
+      move=> _/= /andP[/eqP H2]; rewrite -H2 eqxx/=.
+      apply: IH; auto.
+    move=> LB.
+    case H: (k1 == k); move/eqP: H => H; subst.
+      rewrite lookup_remove_None/= LB/=.
+      rewrite remove2 => H.
+      by rewrite weak2 eqxx orbT/=.
+    rewrite lookup_remove_diff//.
+    case LB1: lookup => //=[vB1|]; last first.
+      rewrite key_absent_remove; last first.
+        by rewrite /key_absent lookup_remove_diff//LB1.
+      have K : key_absent k B by rewrite /key_absent LB1.
+      rewrite (key_absent_remove K).
+      by apply: IH; auto.
+    move=> /andP[].
+    move=> H1; rewrite H1/=.
+    rewrite remove_comm.
+    apply: IH (valid_sig_remove VB) _.
+    rewrite lookup_remove_diff; congruence.
   Qed.
 
-  Lemma lookup_more_precise {k l1 l2 r}:
+
+  (* Lemma lookup_more_precise {k l1 l2 r}:
     lookup k l1 = Some r ->
       more_precise l1 l2 ->
         exists r', lookup k l2 = Some r' /\ incl r r' = ty_ok true.
@@ -1783,7 +1834,7 @@ Section more_precise.
     have [r''[H5 H6]] := IH _ _ _ H1 H4.
     exists r''; split => //.
     rewrite lookup_remove_diff// in H5.
-  Qed.
+  Qed. *)
 
   Lemma lookup_more_precise_None {k l1 l2}:
     valid_sig l2 ->
@@ -1802,18 +1853,26 @@ Section more_precise.
       move=> + /andP[H2 +].
       apply: IH.
     case: eqP => //H LA.
-    case LB: lookup => //=[vB] /andP[/eqP I MP].
+    case LB: lookup => //=[vB|].
+      move=> /andP[I MP].
+      have:= IH _ _ (valid_sig_remove VB) LA MP.
+      rewrite lookup_remove_diff//.
+    move=> MP.
     have:= IH _ _ (valid_sig_remove VB) LA MP.
     rewrite lookup_remove_diff//.
   Qed.
 
-  Lemma more_precise_trans {A B C}:
+  (* Lemma more_precise_trans {A B C}:
     valid_sig C ->
     more_precise A B -> more_precise B C -> more_precise A C.
   Proof.
     elim: A B C => //=[|[k v] A IH] B C VC.
       elim: B C VC => //=[[k v] B IH] C/= VC /andP[/eqP H1 H2].
-      case LC: lookup => //=[vC] /andP[/eqP H3 H4].
+      case LC: lookup => //=[vC|]; last first.
+        move=> _.
+        apply: IH; auto.
+      
+      move=> /andP[/eqP H3 H4].
       apply: IH (VC) (H2) _.
       have Hx:= more_precise_key_absent H4.
       have:= incl_min H3.
@@ -1826,7 +1885,7 @@ Section more_precise.
     rewrite H4 (incl_trans H1 H5)/=.
     apply: IH (valid_sig_remove VC) H2 _.
     by apply: more_precise_remove2.
-  Qed.
+  Qed. *)
 
   Lemma all_weak_all {L}:
     all (fun x => x.2 == weak x.2) (weak_all L).
@@ -1841,25 +1900,82 @@ Section more_precise.
   Lemma lookup_more_precise1 {k l1 l2 r}:
     lookup k l2 = Some r ->
       more_precise l1 l2 ->
-        match lookup k l1 with
-        | Some r' => incl r' r = ty_ok true
-        | None => r = weak r
-        end.
+        r = weak r \/ 
+        exists r', lookup k l1 = Some r' /\ (incl r' r = ty_ok true).
   Proof.
     elim: l1 k l2 r => /=[|[k v] sV IH] k' sV' r L/=.
       move: L; elim: sV' r k'; clear => //=[[k v] A IH r k'].
       case: eqP => //=H; subst.
-        move=> [->]{v}/andP[]/eqP//.
+        move=> [->]{v}/andP[]/eqP//; auto.
       move=> H1 /andP[/eqP H2].
       apply: IH H1.
     case: eqP => H; subst.
-      rewrite L => /andP[/eqP H1 H2]//.
-    case L2: lookup => //=[v1]/andP[/eqP H1 H2].
-    apply: IH H2.
+      rewrite L => /andP[+ H2].
+      move=> /orP[]/eqP; auto.
+      right; repeat eexists; auto.
+    case L2: lookup => //=[v1|]; last first.
+      move=> H1.
+      have:= IH k' _ _ _ H1.
+      rewrite lookup_remove_diff//.
+      by move=> /(_ _ L).
+    move=> /andP[+ MP].
+    have:= IH k' _ _ _ MP.
     rewrite lookup_remove_diff//.
-  Qed.  
+    move=> /(_ _ L) []; auto.
+  Qed.
+
+  Lemma more_precise_trans {A B C}:
+    valid_sig C ->
+    more_precise A B -> more_precise B C -> more_precise A C.
+  Proof.
+    elim: A B C => //=[|[k v] A IH] B C VC.
+      elim: B C VC => //=[[k v] B IH] C/= VC /andP[/eqP H1 H2].
+      case LC: lookup => //=[vC|]; last first.
+        move=> H.
+        rewrite key_absent_remove in H; auto.
+        rewrite/key_absent LC//.
+      move=> /andP[H4 H5].
+      apply: IH; auto.
+      move/orP: H4 => []/eqP H.
+        move: H; rewrite H1.
+        move=> /incl_min; rewrite min_comm.
+        move=> /min_weak1 ?; subst.
+        by apply: more_precise_remove3; eauto.
+      rewrite H in LC.
+      by apply: more_precise_remove3; eauto.
+    case LB: lookup => //=[VB|]; last first.
+      rewrite key_absent_remove/key_absent?LB//.
+      move=> H1 H2.
+      case L: lookup => [vC|].
+        apply: andb_true_intro; split.
+          have:= lookup_more_precise1 L H2.
+          rewrite LB; move=> [<-|[r'[//]]];rewrite eqxx orbT//.
+        apply: IH (valid_sig_remove VC) H1 _.
+        apply: more_precise_removel; auto.
+        by rewrite/key_absent LB.
+      apply: IH (valid_sig_remove VC) H1 _.
+      apply: more_precise_removel; auto.
+      by rewrite/key_absent LB.
+    move=> /andP[] H1 MA MB; case LC: lookup => [vC|]; last first.
+      rewrite key_absent_remove/key_absent?LC//.
+      apply: IH; eauto.
+      apply: more_precise_remover; auto.
+      rewrite/key_absent LC//.
+    apply: andb_true_intro; split.
+      have:= lookup_more_precise1 LC MB.
+      rewrite LB.
+      move=> [].
+        by move=> <-; rewrite eqxx orbT.
+      move=> [r'[[H2] H3]]; subst.
+      move/orP: H1 => []/eqP H.
+        rewrite (incl_trans H H3)//.
+      move: H3; rewrite H => /incl_min; rewrite min_comm.
+      by move=> /min_weak1 <-; rewrite weak2 eqxx orbT.
+    apply: IH (valid_sig_remove VC) MA _.
+    by apply: more_precise_remove2.
+  Qed.
   
-  Lemma lookup_more_precise2 {k l1 l2}:
+  (* Lemma lookup_more_precise2 {k l1 l2}:
     lookup k l2 = None ->
       more_precise l1 l2 ->
         lookup k l1 = None.
@@ -1870,7 +1986,7 @@ Section more_precise.
     case L2: lookup => //=[v1]/andP[/eqP H1 H2].
     apply: IH H2.
     by rewrite lookup_remove_diff.
-  Qed.
+  Qed. *)
 
   Lemma more_precise_refl {s}: 
     valid_sig s -> more_precise s s.
@@ -1881,28 +1997,30 @@ Section more_precise.
   Qed.
 
   Lemma merge_more_precise0 {B C D}:
-    merge_sig B C = ty_ok D ->
+    (* valid_sig B -> valid_sig C -> *)
+    merge_sig B C = D ->
       more_precise B D.
   Proof.
+    (* move=> ++ <-./szz *)
+    move=> <-.
     rewrite merge_comm.
-    elim: B C D => //=[|[k v] B IH] C D/=.
-      rewrite/merge_sig/= weak_bf_merge_0s => -[<-]/=.
+    elim: B C {D} => //=[|[k v] B IH] C /=.
+      rewrite /merge_sig weak_bf_merge_0s/=.
       apply: all_weak_all.
     rewrite/merge_sig/=.
     rewrite (@add_weak_bf_merge _ _ _ _ v)/=?eqxx//.
     rewrite weak_bf_mergeP/=eqxx/=.
-    case L: lookup => [vA|]//=.
-      case M: max => [m|]//=.
+    case LC: (lookup _ C) => [vC|]/=.
       TODO.
     TODO.
   Qed.
 
   (* I *)
 
-  Lemma more_precise_merge1 {A B}:
+  (* Lemma more_precise_merge1 {A B}:
     valid_sig B ->
     more_precise A B -> 
-    exists C, merge_sig A B = ty_ok C.
+    exists C, merge_sig A B = C.
   Proof.
     rewrite merge_comm.
     rewrite/merge_sig.
@@ -1914,12 +2032,12 @@ Section more_precise.
       rewrite (incl_compat_type H1).
       case M: max => //=[m] _.
       rewrite (@add_weak_bf_merge _ _ _ _ v)/=?eqxx//.
-  Abort.
+  Abort. *)
 
   Lemma more_precise_merge {A B C D}:
     valid_sig B -> valid_sig C ->
-    more_precise A B -> merge_sig B C = ty_ok D -> 
-    exists E, merge_sig A C = ty_ok E /\ more_precise E D.
+    more_precise A B -> merge_sig B C = D -> 
+    exists E, merge_sig A C = E /\ more_precise E D.
   Proof.
     rewrite merge_comm (@merge_comm A).
     elim: A B C D => //=[|[k v] A IH] B C D VB VC.
@@ -1929,38 +2047,36 @@ Section more_precise.
       rewrite merge_comm in H2.
       have:=merge_more_precise0 H2.
       TODO.
-    case LB: lookup => //=[vB] /andP[/eqP I H1] H2.
-    rewrite/merge_sig/=.
-    rewrite weak_bf_mergeP/= eqxx.
-    case LC: lookup => [vC|]/=.
+    case LB: lookup => //=[vB|].
+      move=> /andP[I H1] H2.
+      rewrite/merge_sig/=.
+      rewrite weak_bf_mergeP/= eqxx.
+      case LC: lookup => [vC|]/=.
+        TODO.
       TODO.
     TODO.
   Qed.
 
   Lemma more_precise_merge2 {A1 B1 A2 B2 C2}:
     valid_sig A2 -> valid_sig B2 ->
-    more_precise A1 A2 -> more_precise B1 B2 -> merge_sig A2 B2 = ty_ok C2 -> 
-    exists C1, merge_sig A1 B1 = ty_ok C1 /\ more_precise C1 C2.
+    more_precise A1 A2 -> more_precise B1 B2 -> merge_sig A2 B2 = C2 -> 
+    exists C1, merge_sig A1 B1 = C1 /\ more_precise C1 C2.
   Proof.
   Admitted.
 
-  (* THIS IS CLEARLY FALSE *)
-  (* Lemma more_precise_add_None {v sv1 S}:
+  Lemma more_precise_add_None {v sv1 S}:
     valid_sig sv1 ->
     lookup v sv1 = None ->
       more_precise (add v S sv1) sv1.
   Proof.
-    elim: sv1 v S => //=[|[k v] l IH] k' v' /=.
-      (* TODO: IMPORTANT THIS IS TRUE ONLY IF WE CHANGE THE DEF OF MORE PRECISE *)
-      (* NOTE: IF WE CHANGE THE DEFINITION, WE LOOSE THE TRANSITIVITY *)
-      admit.
+    elim: sv1 v S => //=[[k v] l IH] k' v' /=.
     move=>/andP; rewrite/key_absent => -[].
     case L: lookup => []//= _ vl.
     case:eqP => //= H1 H2.
     rewrite eqxx incl_refl//=.
     rewrite key_absent_remove/key_absent?L//.
     by apply: IH.
-  Admitted. *)
+  Qed.
 
   Definition more_precise_opt (more_pre less_pre:((S * bool))) :=
     match less_pre with
@@ -1970,212 +2086,44 @@ Section more_precise.
       end
   end.
 
-  (* Lemma more_precise_check_callable {sP c ctx1 ctx2 s1 s2 b1 b2}:
-    check_callable sP ctx2 c = (s2,b2) ->
-    more_precise ctx1 ctx2 -> valid_sig ctx2 ->
-    (check_callable sP ctx1 c) = (s1,b1) ->
-      (incl s1 s2). *)
-
-  Lemma more_precise_check_tm {sP c ctx1 ctx2 s1 s2 b1 b2}:
-    check_tm sP ctx2 c = (s2,b2) ->
-    more_precise ctx1 ctx2 -> valid_sig ctx2 ->
-    (check_tm sP ctx1 c) = (s1,b1) ->
-      (incl s1 s2 == ty_ok true) || ((s1,b1) == any).
+  Lemma more_precise_get_callable_hd {sP s1 s2 c S}:
+    valid_sig s2 ->
+    more_precise s1 s2 ->
+      get_callable_hd_sig sP s2 c = Some S ->
+        S = weak S \/ 
+        exists S', get_callable_hd_sig sP s1 c = Some S' 
+          /\ incl S' S = ty_ok true.
   Proof.
-    elim: c ctx1 ctx2 s1 s2 b1 b2 => //=.
-    - move=> k ctx1 ctx2 s1 s2 b1 b2.
-      case L: lookup => //=[S|][??] ++ [??]; subst => //.
-      rewrite incl_refl//.
-    - move=> k ctx1 ctx2 s1 s2 b1 b2 [??] ++ [??]; subst => //.
-    - move=> k ctx1 ctx2 s1 s2 b1 b2 + MP V.
-      case L1: lookup => //=[S|][??]; subst.
-        case L2: lookup => //=[S1|][??]; subst.
-          have:= lookup_more_precise1 L1 MP.
-          rewrite L2 => ->//.
-        rewrite eqxx orbT//.
-      rewrite (lookup_more_precise2 L1 MP).
-      move=> [<-<-]; rewrite orbT//.
-    - move=> l Hl r Hr ctx1 ctx2 s1 s2 b1 b2 + MP V.
-      case CL: check_tm => [sl bl].
-      case CR: check_tm => [sr br].
-      case CL1: check_tm => [sl1 bl1].
-      case CR1: check_tm => [sr1 br1].
-      have /orP {}Hl := Hl _ _ _ _ _ _ CL MP V CL1.
-      have /orP {}Hr := Hr _ _ _ _ _ _ CR MP V CR1.
-      move=> {CL CR CL1 CR1}.
-      case: Hl; case: Hr; last first.
-      - move=> /eqP[??]/eqP[??] + <-; subst.
-        by rewrite eqxx orbT.
-      - by move=> + /eqP[??] + <-; subst; rewrite eqxx orbT.
-      - move=> /eqP[??]; subst.
-        case: sl.
-          move=> b + [??]; subst.
-          case: sl1 => //=[|[]]//.
-          move=> b2 + [??]; subst.
-          by rewrite orbT.
-        move=> [] sll slr; case: sl1 => [[]|]//[]//sll1 slr1.
-          
-
-          case: sll1 => //=; last first.
-            move=> m src tgt + + [??]; subst.
-            case E: (incl sr sll); last first.
-              move=> +[??]; subst.
-              have inclR a b c d : incl (a --i--> b) (c --i--> d) = ty_ok true -> incl b d = ty_ok true.
-                by rewrite /incl /=; case: incl_aux; case: incl_aux => //= -[] [].
-              move=> /inclR. move/incl_weak ->.
-              Search incl weak. 
-            rewrite {1}/incl/=.
-          
-          [|move=> m sx sy ++<-; rewrite eqxx orbT//].
-          move=> [|d]//=; [move=> ++<-; rewrite eqxx orbT//|].
-          rewrite andbF/=.
-          move=> ++ [??]; subst.
-          case I: (incl sr) => [b0|]//=; last first.
-            move=> +[??]; subst.
-
-
-          rewrite{2}/incl/=-/incl-/not_incl.
-          rewrite not_incl_incl.
-
-        case: sl.
-          move=> b ++ [??]; subst.
-          case: sl1 => //=[|[]]//.
-          move=> b2 ++ [??]; subst.
-          by rewrite orbT.
-        move=> [] sll slr; case: sl1 => [[]|]//[]//sll1 slr1.
-          rewrite{2}/incl/=-/incl-/not_incl.
-          rewrite not_incl_incl.
-
-
-        move=> []; case: sl1 => //=.
-        case: sl1 => .
-
-          
-          case:
-
-    - move=> k r1 s1 s2 [<-]{r1} H1 H2; repeat eexists.
-    - move=> v [S B] s1 s2.
-      case L: lookup => //=[v1][??]; subst.
-      move=> MP V.
-        (* have [r' [H3 H4]] := lookup_more_precise L H1.
-        rewrite H3//.
-      have:= lookup_more_precise_None H2 L H1. *)
-      case L1: lookup => //=[vs2|]. -> //; rewrite weak2//.
-    - move=> l Hl r Hr sol s1 s2 + H1 H2.
-      case X: (check_tm sP s2 l) => //=[[[S B]|]]//=; last first.
-        move=> [<-]{sol}.
-        have {Hl}[r1[H3 H4]] := Hl _ _ _ X H1 H2.
-        rewrite H3/=.
-        case: r1 H3 H4 => //= H3 _.
-        repeat eexists.
-      case: S X => //= -[] sl sr H.
-        case X: check_tm => //[s3]/=.
-        have {Hl}[r1[H5 H6]] := Hl _ _ _ H H1 H2.
-        case: s3 X => //=[s3|] H3; last first.
-          rewrite H5/=.
-          case: eqP => Hz [<-]{sol}; last first.
-            case: r1 H5 H6 => //=; [|(repeat eexists); rewrite/= weak2//].
-            move=> []//s3 b; rewrite/incl/=.
-            move=> H7 [+ H8].
-            case: s3 H7 H8 => //=.
-              move => []//.
-            have {Hr}[r2[H5 H6]] := Hr _ _ _ H3 H1 H2.
-            move=> []//s3 s4 H4.
-            rewrite -/incl -/not_incl not_incl_incl.
-            rewrite H5/=.
-            case: r2 H5 H6 => /=[[]|]//.
-            move=> H6 H7 H8 H9.
-            move: H8.
-            case I1: incl => /=[[]|]//; case I2: incl => /=[[]|]//= _.
-            case: eqP => Hy; repeat eexists; last first.
-              rewrite (incl_weak I2) incl_refl//.
-            apply: incl_trans I2 _.
-            apply: min_incl.
-            apply: min_weak.
-          case: r1 H5 H6 => //=; last first.
-            repeat eexists; rewrite/=.
-            move: H6 => []//.
-          move=> []//s3 b; rewrite/incl/=.
-          move=> H7 [+ H8].
-          case: s3 H7 H8 => //=.
-            move => []//.
-          have {Hr}[r2[H5 H6]] := Hr _ _ _ H3 H1 H2.
-          move=> []//s3 s4 H4.
-          rewrite -/incl -/not_incl not_incl_incl.
-          rewrite H5/=.
-          case: r2 H5 H6 => /=[[]|]//.
-          move=> H6 H7 H8 H9.
-          move: H8.
-          case I1: incl => /=[[]|]//; case I2: incl => /=[[]|]//= _.
-          move: I1; rewrite Hz.
-          move=> /incl_min; rewrite min_comm.
-          move=> /min_weak1 ?; subst.
-          rewrite weak2 eqxx.
-          by repeat eexists.
-        case: s3 H3 => s3 b1 H3.
-        case I: incl => //=[b][<-]{sol}/=.
-        have {Hr}[r2[H7 H8]] := Hr _ _ _ H3 H1 H2.
-        rewrite H5/= H7/=.
-        case: r1 H5 H6 => //=; last first.
-          move=> H5 [H9]; case: B H => //= H Hz.
-          repeat eexists.
-          by case: ifP => //=; rewrite?weak2//.
-          repeat eexists; rewrite/=weak2//.
-        move=> []/=s4 b2 H4 [].
-        rewrite /incl.
-        (* INPUT CASE *)
-        case: s4 H4 => //=[[]|]//=[]//=s4 s5 H4.
-        rewrite -/incl -/not_incl not_incl_incl.
-        case I1: incl => /=[[]|]//; case I2: incl => /=[[]|]//= + _.
-        case: r2 H7 H8 => //=; last first.
-          move=> H7 H8 H0.
-          case: eqP; repeat eexists; case X: andb => //=.
-          - repeat split.
-            apply: incl_trans I2 _.
-            apply: min_incl min_weak.
-          - destruct b, b1, B => //.
-            have:= incl_trans I I1.
-            rewrite H8.
-            move=> /incl_min; rewrite min_comm => /min_weak1.
-            move=> ?; subst.
-            by rewrite weak2 in n.
-          - rewrite (incl_weak I2) incl_refl//.
-        move=> [s6 b3] H6 [] + H7.
-        have C1 := incl_compat_type I.
-        have C2 := incl_compat_type H7.
-        have C3 := incl_compat_type I1.
-        have {C1 C2 C3} := compat_type_trans1 C2 (compat_type_trans1 C1 C3).
-        rewrite /compat_type.
-        case I3: incl => //=[b4] _ Hz Hy.
-        case Hx: andb; repeat eexists.
-          destruct b2, b3, b4 => //.
-          case Hw: andb => /=; repeat split; auto.
-          apply: incl_trans I2 _.
-          apply: min_incl min_weak.
-        case Hw: andb => //=.
-          destruct B, b1, b => //=.
-          destruct b2, b3 => //=.
-          destruct b4 => //=.
-          have:= incl_trans H7 (incl_trans I I1).
-          congruence.
-        rewrite (incl_weak I2) incl_refl//.
-      have {Hl}[r1[H3 H4]] := Hl _ _ _ H H1 H2.
-      rewrite H3/=.
-      destruct r1; [|repeat eexists]; last first.
-        move: H0; destruct B => -[<-]{sol}//=; rewrite?weak2//=.
-        move: H4 => -[_ <-]//.
-      case: p H3 H4 => /=[s3 b] + [+ ].
-      (* OUTPUT CASE *)
-      case: s3 => [[]|]//=[]//s3 s4 H3 +.
-      rewrite/incl/=.
-      rewrite -/incl -/not_incl.
-      case I1: incl => /=[[]|]//; case I2: incl => /=[[]|]//= + _.
-      destruct b; repeat eexists; move: H0; destruct B => -[<-]{sol}//=; repeat split.
-        apply: incl_trans I2 _.
-        apply: min_incl.
-        apply: min_weak.
-      rewrite (incl_weak I2) incl_refl//.
-  Qed.*)
+    move=> V M.
+    (* have:= more_precise_valid_sig V M. *)
+    rewrite /get_callable_hd_sig/get_tm_hd_sig.
+    case G: get_tm_hd => [E|[P | Var]].
+    - move=> [<-]//; auto.
+    - move=> ->; right; repeat eexists; rewrite incl_refl//.
+    - clear - M s2 V; elim: s1 s2 S Var M V => //=  [|[k v] A IH] B S Var + VB.
+        elim: B {VB} => //= => [[k v] A IH]/= /andP[/eqP H1 H2].
+        case: eqP.
+          move=> _ [] <-; rewrite -H1; auto.
+        move=> H LA.
+        by apply: IH; auto.
+      case LB: lookup => //=[vB|].
+        move=> /andP[I MP].
+        case: eqP => H; subst.
+          rewrite LB => -[?]; subst.
+          move/orP: I => []/eqP H; auto.
+          right; repeat eexists; auto.
+        move=> LB1.
+        apply: IH MP (valid_sig_remove VB) _.
+        rewrite lookup_remove_diff//.
+      move=> MP.
+      case: eqP => H; subst.
+        rewrite LB//.
+      move=> LB1.
+      have:= IH _ _ _ MP (valid_sig_remove VB).
+      move=> /(_ _ Var).
+      rewrite lookup_remove_diff//.
+      by move=> /(_ _ LB1).
+  Qed.
 
   Lemma more_precise_add_Some {v sv1 S S'}:
     valid_sig sv1 ->
@@ -2192,106 +2140,247 @@ Section more_precise.
     by apply: IH; eauto.
   Qed.
 
-  Lemma assume_tm_more_precise {sP sv1 svA c S}:
-    valid_sig sv1 -> assume_tm sP sv1 c S = ty_ok svA -> more_precise svA sv1.
-  Proof.
-    elim: c sv1 svA S => //=.
-    - move=> _ sv1 sv2 _ H [<-]; repeat split => //; apply: more_precise_refl H.
-    - move=> _ sv1 sv2 _ H [<-]; repeat split => //; apply: more_precise_refl H.
-    - move=> v sv1 svA S sv1V.
-      case L: lookup => [S'|]; last first.
-        move=> [<-]/={svA}.
-        (* should be ok under the condition that all var in c in both sv1 and svA *)
-        (* by apply: more_precise_add_None. *)
-        admit.
-      case M: min => //=[S''][<-].
-      apply: more_precise_add_Some; eauto.
-      rewrite min_comm in M.
-      apply: min_incl M.
-    - move=> l Hl r Hr sv1 sv2 [//|[s1 s2|s1 _]] V; last first.
-        by apply: Hl.
-      case al: assume_tm => //[sv1']/= ar.
-      have {}Hl := Hl _ _ _ V al.
-      have V' := assume_tm_valid_sig V al.
-      have {}Hr := Hr _ _ _ V' ar.
-      by apply: more_precise_trans Hr Hl.
-  Admitted.
-
-  Lemma assume_call_more_precise {sP sv1 svA c S}:
+  Lemma more_precise_add_Some1 {v sv1 S S'}:
     valid_sig sv1 ->
-    assume_call sP sv1 c S = ty_ok svA -> 
-      more_precise svA sv1.
+    lookup v sv1 = Some S -> S == weak S ->
+      more_precise (add v S' sv1) sv1.
   Proof.
-    elim: c sv1 svA S => //=.
-    - move=> _ sv1 sv2 _ H [<-]; repeat split => //; apply: more_precise_refl H.
-    - move=> _ sv1 sv2 _ H [<-]; repeat split => //; apply: more_precise_refl H.
-    - move=> c IH t sv1 sv2 []//= m sl s3.
-      case: m; [apply: IH|].
-      case ac: assume_call => //=[sv1'] V.
-      have {}IH := IH _ _ _ V ac.
-      move=> H1.
-      have V' := assume_call_valid_sig V ac.
-      have H2 := assume_tm_more_precise V' H1.
-      by apply: more_precise_trans H2 IH.
+    elim: sv1 v S S' => //=-[k v] l IH k' S S' /= /andP[c vl].
+    case:eqP => //= H; subst.
+      move=> [?]; subst => H.
+      rewrite eqxx/= H/= key_absent_remove// more_precise_refl//orbT//.
+    move=> H1 H2.
+    rewrite eqxx incl_refl/=.
+    rewrite key_absent_remove//.
+    by apply: IH; eauto.
   Qed.
 
-  Lemma more_precise_get_callable_hd {sP s1 s2 c S}:
-    valid_sig s2 ->
-    more_precise s1 s2 ->
-      get_callable_hd_sig sP s2 c = Some S ->
-        match get_callable_hd_sig sP s1 c with
-        | None => S == weak S
-        | Some S' => incl S' S = ty_ok true
-        end.
-  Proof.
-    move=> V M.
-    have:= more_precise_valid_sig V M.
-    rewrite /get_callable_hd_sig/get_tm_hd_sig.
-    case G: get_tm_hd => [E|[P | Var]].
-    - move=> _ [<-]//.
-    - move=> H ->; rewrite incl_refl//.
-    - clear - M s2 V; elim: s1 s2 S Var M V => //=  [|[k v] A IH] B S Var + VB.
-        elim: B {VB} => //= => [[k v] A IH]/= /andP[/eqP H1 H2] _.
-        case: eqP.
-          move=> _ [] <-; rewrite -H1//.
-        move=> H LA.
-        by apply: IH; auto.
-      case LB: lookup => //=[vB] /andP[/eqP I MP].
-      rewrite/key_absent; case LA: lookup => //= VA.
-      case: eqP => H; subst.
-        rewrite LB => -[]<-//.
-      move=> LB1.
-      have {}IH := IH _ _ _ MP (valid_sig_remove VB) VA.
-      apply: IH.
-      rewrite lookup_remove_diff//.
-  Qed.
-
-  Lemma more_precise_get_callable_hd_None {sP s1 s2 c}:
+  (* Lemma more_precise_get_callable_hd_None {sP s1 s2 c}:
     valid_sig s2 ->
     more_precise s1 s2 ->
       get_callable_hd_sig sP s2 c = None ->
         get_callable_hd_sig sP s1 c = None.
   Proof.
     move=> V M.
-    have:= more_precise_valid_sig V M.
+    (* have:= more_precise_valid_sig V M. *)
     rewrite /get_callable_hd_sig/get_tm_hd_sig.
     case G: get_tm_hd => [E|[P | Var]]//.
     clear - M s2 V.
     elim: s1 s2 Var M V => /=[|[k v] A IH] B Var + VB//.
-    case LB: lookup => //=[vB] /andP[/eqP I MP].
-    rewrite/key_absent; case LA: lookup => //= VA.
-    case: eqP => H; subst.
-      congruence.
-    move=> LB1.
-    apply: IH _ _ MP (valid_sig_remove VB) VA _.
-    rewrite lookup_remove_diff//.
+    case LB: lookup => //=[vB|].
+      move=>/andP[/eqP I MP].
+      rewrite/key_absent; case LA: lookup => //= VA.
+      case: eqP => H; subst.
+        congruence.
+      move=> LB1.
+      apply: IH _ _ MP (valid_sig_remove VB) VA _.
+      rewrite lookup_remove_diff//.
+  Qed. *)
+
+  (* VOGLIO QUALCOSA DEL GENERE:
+    f X \/ g X 
+
+    con func f -> func
+    e func g -> (int)
+
+    nella sostituzione risultato dato che non matchano
+    i tipi di X, X non lo assegno.
+
+    La assume_tm non restituisce un opzione, ma direttamente
+    un ctx (quello in entrata nel caso in cui non sia possibilie unificare
+    una signatura con il tipo del termine quando si calcola il min)
+
+    Scritto meglio:
+    - vorrei che assume mi restituisca un contesto più preciso di quello
+      in entrata.
+    - nella merge di due contesti, merge_sig A B = C -> more_precise A C
+    - se more_precise A B -> 
+        more_precise (assume_tm sP s1 tm d) (assume_tm sP s2 tm d)
+    - 
+
+    PB posso avere una variabile X
+    di tipo `Exp` e assumere che abbia tipo `func`.
+    Cosa vuole dire in questo caso essere più preciso?
+    Cosa assegno a X?
+    
+  *)
+
+  (* il problema qui è dato da:
+      tm := X
+      con s1 := {X := func -> func}
+      e s2 := {X := pred}
+      voglio che X diventi un func.
+  *)
+  Lemma more_precise_add_incl {A B k x y}:
+    more_precise A B ->
+      incl x y = ty_ok true ->
+        more_precise (add k x A) (add k y B).
+  Proof.
+    elim: A B k x y => //=.
+      move=> B k x y + H.
+      rewrite lookup_add_same H/=.
+      admit. (*OK*)
+    move=> [k v] A IH B k1 x y.
+    case LB: lookup => [V|].
+      move=> /andP[H1 H2]/= I.
+      case: eqP => H/=; subst.
+        rewrite lookup_add_same/=.
+        rewrite I/=.
+        admit. (*OK*)
+      rewrite lookup_add_diff//;[|congruence].
+      rewrite LB H1/=.
+      admit. (*OK*)
+    move=> MP I/=.
+    case: eqP => H/=; subst.
+      rewrite lookup_add_same/=.
+      rewrite I/=.
+      admit. (*OK*)
+    rewrite lookup_add_diff//;[|congruence].
+    rewrite LB/=.
+    admit. (*OK*)
+  Admitted.
+
+  Lemma more_precise_assume_tm {s1 s2 sP tm d}:
+    valid_sig s1 -> valid_sig s2 ->
+    more_precise s1 s2 ->
+    more_precise (assume_tm sP s1 tm d)
+      (assume_tm sP s2 tm d).
+  Proof.
+    elim: tm s1 s2 d => //=.
+      move=> v s1 s2 d V1 V2 MP.
+      case L2: (lookup _ s2) => [v2|]/=.
+        have [] := lookup_more_precise1 L2 MP.
+          move=> W.
+          case L1: lookup => [v1|]/=.
+            case M1: min => [m1|].
+              case M2: min => [m2|].
+                apply: more_precise_add_incl; auto.
+                admit. (*ok*)
+              apply: more_precise_add_incl; auto.
+              apply: min_incl M1.
+            case M2: min => [m2|].
+              apply: more_precise_add_incl; auto.
+              move: M2.
+              rewrite W => /min_weak1 ->.
+              by apply: incl_refl.
+            by apply: more_precise_add_incl incl_refl.
+          case M1: min => [m1|].
+            apply: more_precise_add_incl; auto.
+            move: M1.
+            rewrite W => /min_weak1 ->.
+            by apply: incl_refl.
+          apply: more_precise_add_incl; auto.
+          apply: incl_refl.
+        move=> [r'[L3 I]].
+        rewrite L3/=.
+        case M1: min => [m1|].
+          case M2: min => [m2|].
+            apply: more_precise_add_incl; auto.
+            admit. (*ok*)
+          have H1 := incl_compat_type I.
+          have H2:= incl_compat_type (min_incl M1).
+          rewrite min_comm in M1.
+          have H3:= incl_compat_type (min_incl M1).
+          have H4 := compat_type_trans1 H3 H1.
+          rewrite compat_type_comm in H2.
+          have := compat_type_trans1 H2 H4.
+          rewrite/compat_type.
+          admit. (*ok*)
+        case M2: min => [m2|].
+          admit. (*ok*)
+        admit. (*ok*)
+      case L1: lookup => [vA|].
+        case M1: min => [m1|].
+          apply: more_precise_add_incl; auto.
+          apply: min_incl M1.
+        apply: more_precise_add_incl; auto.
+        by apply: incl_refl.
+      apply: more_precise_add_incl; auto.
+      by apply: incl_refl.
+    move=> l Hl r Hr s1 s2 d V1 V2 MP.
+    case: d => //.
+    move=> []//=sx sy; auto.
+    (apply: Hr; auto; apply: assume_tm_valid_sig; auto); auto.
+  Admitted. (*OK*)
+
+  Lemma assume_tm_more_precise {sP sv1 svA c S}:
+    valid_sig sv1 -> assume_tm sP sv1 c S = svA -> more_precise svA sv1.
+  Proof.
+    move=> +<-{svA}.
+    elim: c sv1 S => //=.
+    - move=> _ sv1 _; apply: more_precise_refl.
+    - move=> _ sv1 _; apply: more_precise_refl.
+    - move=> v sv1 svA S.
+      case L: lookup => [S'|]; last first.
+        by apply: more_precise_add_None.
+      case M: min => //=[S''|]; subst.
+        apply: more_precise_add_Some; eauto.
+        rewrite min_comm in M.
+        apply: min_incl M.
+      admit.
+    - move=> l Hl r Hr sv1 [_/more_precise_refl//|].
+      move=> [ls rs|ls rh]/= V; auto.
+      have:= Hl sv1 ls V.
+  Admitted.
+
+  Lemma assume_call_more_precise {sP sv1 svA c S}:
+    valid_sig sv1 ->
+    assume_call sP sv1 c S = svA -> 
+      more_precise svA sv1.
+  Proof.
+    move=> H <-{svA}.
+    rewrite/assume_call.
+    apply: assume_tm_more_precise; eauto.
   Qed.
 
-  (* Lemma callable_is_prop {sP s2 c B}:
-    check_tm sP s2 (Callable2Tm c) = (b Exp, B) -> false.
+  Lemma more_precise_check_tm {sP c ctx1 ctx2 s1 s2 b1 b2}:
+    (* valid_sig ctx1 -> valid_sig ctx2 -> *)
+    check_tm sP ctx2 c = (s2,b2) ->
+    more_precise ctx1 ctx2 -> valid_sig ctx2 ->
+    (check_tm sP ctx1 c) = (s1,b1) ->
+      (b1 || ~~b2) /\ (incl s1 s2 = ty_ok true \/ (weak s2 = s2)).
   Proof.
-    elim: c => //=.
-    - move=> k; case: lookup => //=. *)
+    elim: c ctx1 ctx2 s1 s2 b1 b2 => //=.
+    - move=> k ctx1 ctx2 s1 s2 b1 b2.
+      case L: lookup => //=[S|][??] ++ [??]; subst => //=; rewrite incl_refl; auto.
+    - by move=> k ctx1 ctx2 s1 s2 b1 b2 [??] ++ [??]; subst; auto.
+    - move=> k ctx1 ctx2 s1 s2 b1 b2 + MP V.
+      case L1: lookup => //=[S|][??]; subst => /=.
+        case L2: lookup => //=[S1|][??]; subst => /=.
+          have:= lookup_more_precise1 L1 MP.
+          rewrite L2/=.
+          move=> []; auto.
+          by move=> [r'[[?]]]; subst; auto.
+        have:= lookup_more_precise_None V L2 MP.
+        by rewrite L1 => S2; auto.
+      case L2: lookup => [Vk|]/=[??]; subst; auto.
+    move=> l Hl r Hr ctx1 ctx2 s1 s2 b1 b2 + MP V.
+    case CL: check_tm => [sl bl].
+    case CR: check_tm => [sr br].
+    case CL1: check_tm => [sl1 bl1].
+    case CR1: check_tm => [sr1 br1].
+    have [B1 {}Hl] := Hl _ _ _ _ _ _ CL MP V CL1.
+    have [B2 {}Hr] := Hr _ _ _ _ _ _ CR MP V CR1.
+    case: Hl => []; case: Hr => []; subst; last first.
+    - 
+      (* move=> {CL CR CL1 CR1}. *)
+      move=> H1 H2.
+      rewrite-H1-H2.
+      case: sl CL H2 => //=.
+        move=> [|d]/=CL H2[??]; subst => /=.
+          case: sl1 CL1 => /=.
+            by move=> bb CL1 [??]; subst; auto.
+          move=> [] S1 S2/=; last first.
+            move=> CL1 [??]; subst.
+            admit.
+          admit.
+        case: sl1 CL1 => /=.
+          by move=> bb CL1 [??]; subst; auto.
+        move=> [] S1 S2/=; last first.
+          move=> CL1 [??]; subst.
+          destruct d => //=.
+  Admitted. (*TODO*)
+
 
   Lemma more_precise_check_callable {sP s1 s2 c d0 d' dc sA}:
     check_callable sP s2 c d0 = (dc, sA) -> minD d' d0 = d' ->
@@ -2312,12 +2401,11 @@ Section more_precise.
         move=> d H.
         case: B1 H => H; [|repeat eexists; auto].
         case G: get_callable_hd_sig => //=[S|]; [|repeat eexists; auto].
-        case A: assume_call; repeat eexists; auto.
+        repeat eexists.
           rewrite minD_comm//.
-        apply: more_precise_trans MP.
-          admit. (*valid*)
-        apply: assume_call_more_precise A.
-        admit. (*valid*)
+        apply: more_precise_trans MP; auto.
+        apply: assume_call_more_precise; eauto.
+        vst.
       move=> d.
       case: B; last first.
         move=> H [??] H1 H2 H3; subst.
@@ -2326,71 +2414,99 @@ Section more_precise.
         move=> D; case: B1; [|repeat eexists; auto].
         move=> H4.
         case G: get_callable_hd_sig; [|repeat eexists; auto].
-        case A: assume_call; repeat eexists; auto.
+        repeat eexists; auto.
           by rewrite minD_comm.
-        apply: more_precise_trans H2.
-          admit. (*valid*)
-        apply: assume_call_more_precise A.
-        admit. (*valid*)
-      case G1: get_callable_hd_sig; last first.
-        move=> H [??] M MP V; subst.
-        case: S1 C1; last first.
-          by repeat eexists; auto.
-        move=> []; [repeat eexists; auto|].
-        move=> d1.
-        case: B1 => H1; [|repeat eexists; auto].
-        case G: get_callable_hd_sig => //=[S|]; [|repeat eexists; auto].
-        case A: assume_call; repeat eexists; auto.
-          rewrite minD_comm//.
-        apply: more_precise_trans MP.
-          admit. (*valid*)
-        apply: assume_call_more_precise A.
-        admit. (*valid*)
-      case A: assume_call; last first.
-        move=> H1 [??] M MP V; subst.
-        case: S1 C1; last first.
-          by repeat eexists; auto.
-        move=> []; [repeat eexists; auto|].
-        move=> d1.
-        case: B1 => H2; [|repeat eexists; auto].
-        case G: get_callable_hd_sig => //=[S|]; [|repeat eexists; auto].
-        case A1: assume_call; repeat eexists; auto.
-          rewrite minD_comm//.
-        apply: more_precise_trans MP.
-          admit. (*valid*)
-        apply: assume_call_more_precise A1.
-        admit. (*valid*)
-      move=> H [??] M MP V; subst.
-      case: S1 C1; last first.
-        move=> m s3 s4 H1.
-        
-        ; repeat eexists.
-
-        admit. (*should be false: not arr in conclusion*)
-      move=> [|d1] H1.
-        admit. (*should be false exp in conclusion*)
-      case: B1 H1 => H1; last first.
-        admit. (*should be false: the bool in H is true and in H2 is false*)
-      case G2: get_callable_hd_sig => [SHD|]; last first.
-        (* should be False: if head of G2 is ty_err then H2 should be (_, false) *)
+        apply: more_precise_trans H2; auto.
+        apply: assume_call_more_precise; eauto.
+        vst.
+      move=> C2 + M MP V.
+      have:= more_precise_check_tm C2 MP V C1.
+      move=> []/=.
+      destruct B1 => //= _.
+      move=> [].
+        case: S1 C1 => [|[]]//[]//d1 C1 I.
+        rewrite/get_callable_hd_sig/get_tm_hd_sig.
+        case H: get_tm_hd => [D|[P|EV]]/=.
+        - move=> [??]; subst; repeat eexists.
+            by destruct d', d0, d, d1 => //=.
+          rewrite/assume_call.
+          apply: more_precise_assume_tm; auto.
+          vst.
+        - case L: lookup => [vP|][??]; subst; repeat eexists; auto.
+            by destruct d', d0, d, d1 => //=.
+          apply: more_precise_assume_tm; auto.
+          vst.
+        case L1: lookup => [V1|][??]; subst.
+          (* Search more_precise lookup. *)
+          have:= lookup_more_precise1 L1 MP.
+          move=> [].
+            move=> H1.
+            rewrite H1/=.
+            case L2: lookup => [V2|]/=; repeat eexists.
+            - by destruct d', d0, d, d1 => //=.
+            - admit.
+            - destruct d, d0, d', d1 => //=.
+              (*I think that, since the head is weak in C2 is weak, then it returns Pred*)
+              admit.
+            - admit.
+          move=> [r'[H1 H2]].
+          rewrite H1; repeat eexists.
+            destruct d, d0, d', d1 => //=.
+          admit.
+        case L2: lookup => [V2|]/=; repeat eexists; auto.
+          by destruct d, d0, d', d1 => //=.
         admit.
-      case A1: assume_call; last first.
-        (* hope: assume in A1 should not be ty-err *)
+      move=> []; destruct d => //= H.
+      rewrite/get_callable_hd_sig/get_tm_hd_sig.
+      case H1: get_tm_hd => [D|[P|EV]]/=.
+      - move=> [??]; subst.
+        case: S1 C1.
+          move=> [|d]/= C1.
+            repeat eexists; auto.
+            admit.
+          repeat eexists; [rewrite minD_comm//|].
+          apply: more_precise_assume_tm; auto.
+          vst.
         admit.
-      repeat eexists; auto.
-        rewrite minD_comm.
-        destruct d,d0 => //=.
-        destruct d' => //=.
-        (* d1 should be Func from H2 and H *)
+      - case L: lookup => [vP|][??]; subst.
+          case: S1 C1.
+            move=> [|d]/= C1.
+              repeat eexists; auto.
+              admit.
+            repeat eexists; [rewrite minD_comm//|].
+            apply: more_precise_assume_tm; auto.
+            vst.
+          repeat eexists; auto.
+          admit.
+        case: S1 C1.
+          move=> [|d]/= C1; by repeat eexists; auto.
+        by repeat eexists; auto.
+      case L1: lookup => [V1|][??]; subst.
+        have:= lookup_more_precise1 L1 MP.
+        move=> [].
+          move=> H2.
+          rewrite H2/=.
+          admit.
+        move=> [r'[H2 H3]].
+        rewrite H2.
         admit.
-      (*hope it is true*)
       admit.
-    move=> m s3 s4 H2 [??] M MP V; subst.
-    destruct S1; [|repeat eexists; auto].
-    destruct b;[repeat eexists; auto|].
-    destruct B1; [|repeat eexists; auto].
-    (* should be False: from C1 and H2 *)
-    admit. 
+    move=> m l r C2 [??] M MP V; subst.
+    have:= more_precise_check_tm C2 MP V C1.
+    admit.
+  Admitted.
+
+  Lemma more_precise_merge_sig2 {sA' sB' sVA sVB}:
+    more_precise sA' sVA ->
+    more_precise sB' sVB ->
+    more_precise (merge_sig sA' sB') (merge_sig sVA sVB).
+  Proof.
+  Admitted.
+
+  Lemma more_precise_merge_sig3 {sA' sVA sVB}:
+    more_precise sA' sVA ->
+    more_precise sA' (merge_sig sVA sVB).
+  Proof.
   Admitted.
 
   Lemma more_precise_tc_tree_aux {sP A s1 s2 d0 dA sA d'}:
@@ -2420,40 +2536,35 @@ Section more_precise.
       case: ifP => DB.
         move=> H.
         by apply: HA; eauto.
-      case dtA: (tc_tree_aux _ _ A) => //=[dA' svA].
+      case dtA: (tc_tree_aux _ _ A) => //=[dA' sVA].
       case dtB: (tc_tree_aux _ _ B) => //=[dB sVB].
       have {HA}[dA''[sA'[H3 [H4 H5]]]]:= HA _ _ _ _ _ _ V dtA H1 H2.
       have {HB}[dB''[sB'[H6 [H7 H8]]]]:= HB _ _ _ _ _ _ V dtB H1 H2.
       rewrite H4 H7/=.
       have VA := tc_tree_aux_valid_sig V dtA.
       have VB := tc_tree_aux_valid_sig V dtB.
-      case M: merge_sig => //= [m|] [??]; subst.
-        have [E[M1 H9]] := more_precise_merge2 VA VB H5 H8 M.
-        rewrite M1/=; repeat eexists; auto.
-        case: ifP => //=.
-        rewrite minD_comm; destruct dA', dB => //=.
-        destruct dA'', dB'' => //.
-      admit.
-      
+      move=> [??]; subst.
+      repeat eexists.
+        case: ifP; destruct dA', dB, dA'', dB'' => //.
+      by apply: more_precise_merge_sig2.
     - move=> A HA B0 HB0 B HB s1 s2 d0 dA sA d' V.
       case:ifP => kA.
         move=> [??]; subst.
         by repeat eexists; auto.
-      case dtA: (tc_tree_aux _ _ A) => //=[dA' svA].
+      case dtA: (tc_tree_aux _ _ A) => //=[dA' sVA].
       case dtB0: (tc_tree_aux _ _ B0) => //=[dB0 sVB0].
       case dtB: (tc_tree_aux _ _ B) => //=[dB sVB].
-      case M: merge_sig => //=[m|][??]; subst => H1 H2.
-        have {HA}[dA''[sA'[H3 [H4 H5]]]] := HA _ _ _ _ _ _ V dtA H1 H2.
-        have VA := tc_tree_aux_valid_sig V dtA.
-        have {HB0}[dB0'[sB0'[H6 [H7 H8]]]] := HB0 _ _ _ _ _ _ VA dtB0 H3 H5.
-        have {HB}[dB'[sB'[H9 [H10 H11]]]] := HB _ _ _ _ _ _ VA dtB H3 H5.
-        rewrite H4 H7 H10/=.
-        have VB := tc_tree_aux_valid_sig VA dtB.
-        have VB0 := tc_tree_aux_valid_sig VA dtB0.
-        have [E[M1 H12]] := more_precise_merge2 VB VB0 H11 H8 M.
-        rewrite M1/=; repeat eexists; eauto.
-        rewrite minD_comm; destruct dB0, dB, dB0', dB' => //.
-      
+      move=> [H?] H1 H2; subst.
+      have {HA}[dA''[sA'[H3 [H4 H5]]]] := HA _ _ _ _ _ _ V dtA H1 H2.
+      have VA := tc_tree_aux_valid_sig V dtA.
+      have {HB0}[dB0'[sB0'[H6 [H7 H8]]]] := HB0 _ _ _ _ _ _ VA dtB0 H3 H5.
+      have {HB}[dB'[sB'[H9 [H10 H11]]]] := HB _ _ _ _ _ _ VA dtB H3 H5.
+      rewrite H4 H7 H10/=.
+      have VB := tc_tree_aux_valid_sig VA dtB.
+      have VB0 := tc_tree_aux_valid_sig VA dtB0.
+      repeat eexists.
+        destruct dB0, dB, dB0', dB' => //.
+      by apply: more_precise_merge_sig2.
   Qed.
   Print Assumptions more_precise_tc_tree_aux.
 End more_precise.
@@ -2467,69 +2578,67 @@ Section same_ty.
     (map_ty' F A) == (map_ty' F B). 
 
   Lemma same_ty_subst_check_callable sP sV c D1 D2:
-    same_ty snd (check_callable sP sV c D1) (check_callable sP sV c D2).
+    snd (check_callable sP sV c D1) = snd (check_callable sP sV c D2).
   Proof.
     rewrite/check_callable/=/same_ty.
-    case X: check_tm => [[[[[|bb]|] []]|]|]//=.
+    case X: check_tm => [[[//|D3] [|//]|//]].
     case Y: get_callable_hd_sig => [s2|]//=.
-    case Z: assume_call => //=.
   Qed.
 
   Lemma same_ty_tc_tree_aux sP sV A d1 d2:
-    same_ty snd (tc_tree_aux sP sV A d1) (tc_tree_aux sP sV A d2).
+    snd (tc_tree_aux sP sV A d1) = snd (tc_tree_aux sP sV A d2).
   Proof.
     rewrite/same_ty.
     elim: A d1 d2 sV => //=.
     - move=> _ c d1 d2 sV.
       have:= same_ty_subst_check_callable sP sV c d1 d2.
-      by do 2 case: check_callable => [[]|]//=.
+      by do 2 case: check_callable.
     - move=> A HA s B HB d1 d2 sV.
       case:ifP => dA.
         apply: HB.
       case:ifP => dB.
         apply: HA.
       have {HA} := HA d1 d2 sV.
-      case X: tc_tree_aux => //=[[x y]|]; case Y: tc_tree_aux => /=[[z w]|]//=.
-      move=> /eqP[?]; subst.
+      case X: tc_tree_aux => //=[x y]; case Y: tc_tree_aux => /=[z w]?; subst.
       have {HB} := HB d1 d2 sV.
-      case Z: tc_tree_aux => //=[[a b]|]; case T: tc_tree_aux => /=[[c d]|]//=.
-      move=> /eqP[?]; subst.
+      case Z: tc_tree_aux => //=[a b]; case T: tc_tree_aux => /=[c d]?; subst.
       case M: merge_sig => //=.
     - move=> A HA B0 HB0 B HB d1 d2 sV.
       case:ifP => kA.
         rewrite//=eqxx.
       have {HA} := HA d1 d2 sV.
-      case: (tc_tree_aux _ _ A) => /=[[dA sA]|]//;
-      case: (tc_tree_aux _ _ A) => /=[[dA' sA']|]//; last first.
-      move=>/eqP[->].
+      case: (tc_tree_aux _ _ A) => /=[dA sA]//;
+      case: (tc_tree_aux _ _ A) => /=[dA' sA']//?; subst.
       have {HB0}/= := HB0 dA dA' sA'.
-      case dtB0: (tc_tree_aux _ _ B0) => //=[[x y]|]; case dtB0': (tc_tree_aux _ _ B0) => /=[[z w]|]//=; repeat case: ifP => //.
-      move=> /eqP[?]; subst.
+      case dtB0: (tc_tree_aux _ _ B0) => //=[x y]; case dtB0': (tc_tree_aux _ _ B0) => /=[z w]//=?; subst.
       have {HB}/= := HB dA dA' sA'.
-      case dtB: tc_tree_aux => //=[[a b]|]; case dtB': tc_tree_aux => /=[[c d]|]//=; repeat case: ifP => //=.
-      move=> /eqP[?]; subst.
+      case dtB: tc_tree_aux => //=[a b]; case dtB': tc_tree_aux => /=[c d]//=?; subst.
       case X: merge_sig => //=.
   Qed.
 
   Lemma same_ty_subst_check_callable1 {sP sV A d1 D1 S} d2:
-    check_callable sP sV A d1 = ty_ok (D1, S) ->
+    check_callable sP sV A d1 = (D1, S) ->
       minD d2 d1 = d2 ->
-        exists D2, check_callable sP sV A d2 = ty_ok (D2, S) /\ minD D2 D1 = D2.
+        exists D2, check_callable sP sV A d2 = (D2, S) /\ minD D2 D1 = D2.
   Proof.
     rewrite/check_callable/=.
-    case X: check_tm => [[[[[|bb]|] []]|]|]//=.
-    - case G: get_callable_hd_sig => [s2|]; [|move=> [??]H; subst; repeat eexists].
-      case Z: assume_call => //=[S1][??] H; subst; repeat eexists.
-      destruct bb => //=.
-    - move=> [??] H; subst; repeat eexists.
-    - case G: get_callable_hd_sig => [s2|]; [|move=> [??]H; subst; repeat eexists].
-      case Z: assume_call => //=[S1][??] H; subst; repeat eexists.
+    case X: check_tm => [[d|m l r] b]; last first.
+      move=> [??]; subst; repeat eexists.
+    case: d X.
+      move=> +[??]; subst; repeat eexists.
+    case: b; last first.
+      move=> d + [??]; subst; repeat eexists; auto.
+    move=> d H.
+    case G: get_callable_hd_sig => [s2|]; [|move=> [??]; subst; repeat eexists].
+    move=> [??] H1; subst.
+    repeat eexists.
+    by destruct d, d1, d2.
   Qed.
 
   Lemma same_ty_tc_tree_aux1 {sP sV A d1 D1 S} d2:
-    tc_tree_aux sP sV A d1 = ty_ok (D1, S) ->
+    tc_tree_aux sP sV A d1 = (D1, S) ->
       minD d2 d1 = d2 ->
-        exists D2, tc_tree_aux sP sV A d2 = ty_ok (D2, S) /\ minD D2 D1 = D2.
+        exists D2, tc_tree_aux sP sV A d2 = (D2, S) /\ minD D2 D1 = D2.
   Proof.
     elim: A sV d1 d2 D1 S => //=.
     - move=> sV d1 d2 D1 S [??] <-; subst; repeat eexists.
@@ -2539,7 +2648,7 @@ Section same_ty.
     - move=> sV d1 d2 D1 S [??] <-; subst; repeat eexists.
       rewrite -minD_assoc minD_refl//.
     - move=> _ c d1 d2 sV D1 S.
-      case C: check_callable => //=[[D V]][??] H; subst.
+      case C: check_callable => //=[D V][??] H; subst.
       have [D2[H1 H2]] := same_ty_subst_check_callable1 C H.
       rewrite H1; repeat eexists.
       destruct D2, D, sV, d2 => //=.
@@ -2549,23 +2658,23 @@ Section same_ty.
         apply: HB.
       case:ifP => dB.
         apply: HA.
-      case X: tc_tree_aux => //=[[x y]|]; case Y: tc_tree_aux => /=[[z w]|]//=.
-      case M: merge_sig => //=[m][<-]{D1}? H; subst.
-      have [D3 [dtA Hx]] := HA _ _ _ _ _ Y H.
-      have [D4 [dtB Hy]] := HB _ _ _ _ _ X H.
-      rewrite dtA dtB/= M/=; repeat eexists; case: ifP => //=.
+      case X: tc_tree_aux => //=[x y]; case Y: tc_tree_aux => /=[z w]//=.
+      move=> [??]H; subst.
+      have [D3 [dtA Hx]] := HA _ _ _ _ _ X H.
+      have [D4 [dtB Hy]] := HB _ _ _ _ _ Y H.
+      rewrite dtA dtB/=; repeat eexists; case: ifP => //=.
       destruct D4, D3, z, x => //=.
     - move=> A HA B0 HB0 B HB d1 d2 sV D1 S.
       case:ifP => kA.
         move=> [??]; subst.
         by repeat eexists.
-      case dtA: (tc_tree_aux _ _ A) => /=[[dA sA]|]//.
-      case dtB0: (tc_tree_aux _ _ B0) => //=[[x y]]; case dtB: (tc_tree_aux _ _ B) => /=[[z w]|]//=.
-      case X: merge_sig => //=[m] [?? H]; subst.
+      case dtA: (tc_tree_aux _ _ A) => /=[dA sA]//.
+      case dtB0: (tc_tree_aux _ _ B0) => //=[x y]; case dtB: (tc_tree_aux _ _ B) => /=[z w].
+      move=> [??]H; subst.
       have [D3[dtA' Hx]] := HA _ _ _ _ _ dtA H.
       have [D4[dtB0' Hy]] := HB0 _ _ _ _ _ dtB0 Hx.
       have [D5[dtB' Hz]] := HB _ _ _ _ _ dtB Hx.
-      rewrite dtA' dtB0' dtB'/= X/=; repeat eexists.
+      rewrite dtA' dtB0' dtB'/=/=; repeat eexists.
       destruct D4, D5, x, z => //.
   Qed.
 
@@ -2575,7 +2684,7 @@ Section dead_cutr_cutl.
 
   Lemma is_ko_tc_tree_aux {sP sV A d}:
     valid_sig sV -> is_ko A ->
-    tc_tree_aux sP sV A d = ty_ok(d, sV).
+    tc_tree_aux sP sV A d =(d, sV).
   Proof.
     elim: A sV d=> //=; try by eexists.
     - move=> A HA s B HB sV d H /andP[kA kB].
@@ -2586,7 +2695,7 @@ Section dead_cutr_cutl.
 
   Lemma cutr_tc_tree_aux {sP sV A d}:
     valid_sig sV ->
-    tc_tree_aux sP sV (cutr A) d = ty_ok(d, sV).
+    tc_tree_aux sP sV (cutr A) d =(d, sV).
   Proof.
     move=> H.
     apply: is_ko_tc_tree_aux => //.
@@ -2595,7 +2704,7 @@ Section dead_cutr_cutl.
 
   Lemma is_dead_tc_tree_aux {sP sV A d}:
     valid_sig sV ->
-    tc_tree_aux sP sV (dead A) d = ty_ok(d, sV).
+    tc_tree_aux sP sV (dead A) d =(d, sV).
   Proof.
     move=> H.
     apply: is_ko_tc_tree_aux => //.
@@ -2604,7 +2713,7 @@ Section dead_cutr_cutl.
 
   Lemma cutl_tc_tree_aux {sP sV A d}:
     valid_sig sV -> success A ->
-    tc_tree_aux sP sV (cutl A) d = ty_ok(d, sV).
+    tc_tree_aux sP sV (cutl A) d =(d, sV).
   Proof.
     elim: A sV d => //=.
     - move=> A HA s B HB sV d V; case: ifP => [dA sB|dA sA]/=.
@@ -2619,7 +2728,7 @@ End dead_cutr_cutl.
 
 Section next_alt.
   Lemma success_det_tree_next_alt {sP A sV1 sV2 ign}:
-    success A -> (tc_tree_aux sP sV1 A ign) = ty_ok (Func, sV2) ->
+    success A -> (tc_tree_aux sP sV1 A ign) = (Func, sV2) ->
       (ign = Func /\ next_alt false (build_na A (next_alt true A)) = None)%type2.
   Proof.
     simpl in sV2.
@@ -2636,10 +2745,9 @@ Section next_alt.
         rewrite ?is_dead_next_alt ?is_dead_dead//.
       rewrite success_is_ko//=.
       case: ifP => kB; last first.
-        case dtA: (tc_tree_aux _ _ A) => //=[[dA svA]].
-        case dtB: (tc_tree_aux _ _ B) => //=[[dB sVB]].
-        case M: merge_sig => //= [m] [+?]; subst.
-        rewrite success_has_cut//.
+        case dtA: (tc_tree_aux _ _ A) => //=[dA svA].
+        case dtB: (tc_tree_aux _ _ B) => //=[dB sVB].
+        by rewrite success_has_cut.
       move=> tcA.
       have [? {}HA] := HA _ _ _ sA tcA; subst; repeat split.
       rewrite (is_ko_next_alt _ kB)/=.
@@ -2651,10 +2759,9 @@ Section next_alt.
       have fA := success_failed _ sA.
       have fB := success_failed _ sB.
       rewrite fA/= sA/=.
-      case dA: (tc_tree_aux _ _ A) => //=[[DA sVA]].
-      case dB0: (tc_tree_aux _ _ B0) => //=[[DB0 sVB0]].
-      case dB: (tc_tree_aux _ _ B) => //=[[DB sVB]].
-      case M: merge_sig => //=[S][??]; subst.
+      case dA: (tc_tree_aux _ _ A) => //=[DA sVA].
+      case dB0: (tc_tree_aux _ _ B0) => //=[DB0 sVB0].
+      case dB: (tc_tree_aux _ _ B) => //=[DB sVB].
       destruct DB0, DB => //=.
       have {HB} [?]:= HB _ _ _ sB dB; subst.
       have {HA} [?]:= HA _ _ _ sA dA; subst.
@@ -2672,15 +2779,15 @@ Section next_alt.
 
   Lemma failed_det_tree_next_alt {sP A sV1 sV2 d ign B} b:
     valid_sig sV1 ->
-    tc_tree_aux sP sV1 A ign = ty_ok (d, sV2) ->
+    tc_tree_aux sP sV1 A ign = (d, sV2) ->
       next_alt b A = Some B ->
         exists d' sv2', minD d' d = d' /\ 
-          (tc_tree_aux sP sV1 B ign) = ty_ok (d', sv2') /\ more_precise sv2' sV2.
+          (tc_tree_aux sP sV1 B ign) = (d', sv2') /\ more_precise sv2' sV2.
   Proof.
     elim: A B sV1 sV2 d ign b => //=.
     - move=> B s1 s2 d ign []//= V [??][?]; subst; repeat eexists; rewrite ?minD_refl//?less_precise1_refl//?merge_refl//?more_precise_refl//.
-    - move=> p c B s1 s2 d1 d2 _ V. 
-      case C: check_callable => //= [[D S]][??][?]; subst => /=.
+    - move=> p c B s1 s2 d1 d2 _ V.
+      case C: check_callable => //= [D S][??][?]; subst => /=.
       rewrite C.
       have?:= (check_callable_valid_sig V C).2.
       repeat eexists; rewrite ?minD_refl//?less_precise1_refl//?merge_refl//=?more_precise_refl//.
@@ -2702,11 +2809,11 @@ Section next_alt.
         case nA: next_alt => //=[A'][<-]{s1}/=.
         rewrite (next_alt_is_ko nA) kB.
         by apply: HA; eauto.
-      case dtA: (tc_tree_aux _ _ A) => /=[[DA sVA]|]//=.
+      case dtA: (tc_tree_aux _ _ A) => /=[DA sVA]//=.
       have VA := tc_tree_aux_valid_sig V dtA.
-      case dtB: (tc_tree_aux _ _ B) => /=[[DB sVB]|]//=.
+      case dtB: (tc_tree_aux _ _ B) => /=[DB sVB]//=.
       have VB := tc_tree_aux_valid_sig V dtB.
-      case M: merge_sig => //=[m][??]; subst.
+      move=> [??]; subst.
       case nA: next_alt => [A'|]//=.
         move=> [?]; subst.
         have:= HA _ _ _ _ _ _ V dtA nA.
@@ -2714,11 +2821,12 @@ Section next_alt.
         rewrite tcA'/= dtB/=.
         have VS:= tc_tree_aux_valid_sig V tcA'.
         rewrite (has_cutF_next_alt nA).
-        have [X[M1 L2]] := more_precise_merge VA VB L M.
-        rewrite (next_alt_is_ko nA)/=M1/=.
+        rewrite (next_alt_is_ko nA)/=.
         rewrite kB.
         (repeat eexists) => //=.
-        by case:ifP => //=; destruct d', DA, DB => //.
+          by case:ifP; destruct d', DA, DB.
+        apply: more_precise_merge_sig2; auto.
+        by apply: more_precise_refl.
       case nB: next_alt => [B'|]//=.
       have {HB}:= HB _ _ _ _ _ _ V dtB nB.
       move => -[d'[S [m [dtB' L]]]] [?]; subst.
@@ -2729,21 +2837,18 @@ Section next_alt.
         destruct d' => //.
       have /=H := @is_dead_tc_tree_aux sP s2 A d2 V.
       have VS := tc_tree_aux_valid_sig V dtB'.
-      have L1 := tc_tree_aux_less_precise V dtB'.
-      rewrite merge_comm in M.
-      have:= merge_more_precise0 M.
-      apply: more_precise_trans; auto.
-      apply: merge_sig_valid_sig VB VA M.
+      rewrite merge_comm.
+      by apply: more_precise_merge_sig3.
     move=> A HA B0 HB0 B HB C s1 s2 d1 d2 b V.
     case: ifP => kA.
       by rewrite is_ko_failed//is_ko_next_alt//=.
-    case dtA: (tc_tree_aux _ _ A) => /=[[DA sVA]|]//=.
+    case dtA: (tc_tree_aux _ _ A) => /=[DA sVA]//=.
     have VA := tc_tree_aux_valid_sig V dtA.
-    case dtB0: (tc_tree_aux _ _ B0) => /=[[DB0 sVB0]|]//=.
+    case dtB0: (tc_tree_aux _ _ B0) => /=[DB0 sVB0]//=.
     have VB0 := tc_tree_aux_valid_sig VA dtB0.
-    case dtB: (tc_tree_aux _ _ B) => /=[[DB sVB]|]//=.
+    case dtB: (tc_tree_aux _ _ B) => /=[DB sVB]//=.
     have VB := tc_tree_aux_valid_sig VA dtB.
-    case M: merge_sig => //=[m][??]; subst.
+    move=> [??]; subst.
     case:ifP => fA.
       case nA: next_alt => //=[A'].
       case nB0: next_alt => //=[B0'][<-]{C}/=.
@@ -2760,25 +2865,23 @@ Section next_alt.
       repeat eexists; eauto.
         rewrite minD_comm; destruct DB0, DB, dA', dA'' => //=.
         by destruct dx; simpl in *.
-
-      rewrite merge_comm in M.
-      have:= merge_more_precise0 M.
-      apply: more_precise_trans => //.
-      apply: merge_sig_valid_sig M; auto.
+      by rewrite merge_comm; apply: more_precise_merge_sig3; auto.
     case: ifP => sA; last first.
-      move=> [<-]{C}/=; rewrite dtA/= dtB0 dtB/= M/=.
+      move=> [<-]{C}/=; rewrite dtA/= dtB0 dtB/=.
       rewrite failed_is_ko//.
-      have ? := merge_sig_valid_sig VB VB0 M.
-      by repeat eexists; rewrite ?minD_refl//?more_precise_refl//=.
+      (* have ? := merge_sig_valid_sig VB VB0 M. *)
+      repeat eexists; rewrite ?minD_refl//?more_precise_refl//=.
+      vst.
     case nB: next_alt => //=[B'|].
       move=> [<-]{C}/=.
       rewrite dtA/=kA.
       have:= HB _ _ _ _ _ _ VA dtB nB.
       move=>[d'[S [m [tcB' L]]]]/=.
       rewrite tcB'/= dtB0/=.
-      have/=[E[M1 L1]] := more_precise_merge VB VB0 L M.
-      rewrite M1/=; repeat eexists; auto.
-      by destruct DB0, d', DB => //.
+      repeat eexists.
+        by destruct DB0, d', DB => //.
+      apply: more_precise_merge_sig2; auto.
+      by rewrite more_precise_refl.
     case nA: next_alt => //=[A'].
     case nB0: next_alt => //=[B0'][<-]{C}/=.
     have:= HA _ _ _ _ _ _ V dtA nA.
@@ -2792,14 +2895,11 @@ Section next_alt.
     have Z := more_precise_trans VB0 H3' Hy.
     have [E[Hr Hs]]:= more_precise_merge2 VB0 VB0 Z H3 (merge_refl VB0).
     rewrite Hr/= (next_alt_is_ko nA).
-    repeat eexists; eauto.
+    repeat eexists.
       rewrite minD_comm; destruct DB0, DB, dA', dA'' => //=.
       by destruct dx; simpl in *.
-
-    rewrite merge_comm in M.
-    have:= merge_more_precise0 M.
-    apply: more_precise_trans => //.
-    apply: merge_sig_valid_sig M; auto.
+    rewrite merge_comm.
+    by apply: more_precise_merge_sig3.
   Qed.
   Print Assumptions failed_det_tree_next_alt.
 
@@ -2814,9 +2914,9 @@ Fixpoint sigma2ctx (sP:sigT) (s: Sigma) : option sigV :=
     | None => None
     | Some S =>
         match check_tm sP empty_ctx v with
-        | ty_err => None
-        | ty_ok None => Some S
-        | ty_ok (Some (v, b1)) => Some (add k (if b1 then v else weak v) S)
+        (* | ty_err => None *)
+        (* | None => Some S *)
+        | ((v, b1)) => Some (add k (if b1 then v else weak v) S)
         end
       end
   end.
@@ -2827,7 +2927,7 @@ Proof.
   elim: s S => [[]|]//[k v] xs IH S/=.
   case X: sigma2ctx => //=[S'].
   have {}IH := IH _ X.
-  case C: check_tm => //=[[[k' v']|]]//=; try congruence.
+  case C: check_tm => //=[k' v']//=; try congruence.
   move=> []?; subst.
   by apply: valid_sig_add.
 Qed.
@@ -2839,7 +2939,7 @@ Lemma check_rules_select {sP sV u l rc m s rules}:
 Proof.
   move=> +<-{l}.
   elim: rules => //= -[hd pm]/= rs IH.
-  case cr: check_rule => [[]|]//= /IH {}IH.
+  case cr: check_rule => []//= /IH {}IH.
   case X: H => //=[s']; rewrite IH andbT.
   rewrite cr//.
 Qed.
